rewrite mult and add

code/experimental/rsa/Hacl.Impl.Addition.fst
@@ -13,24 +13,23 @@ val bn_sub_:
     #aLen:size_nat -> #bLen:size_nat ->
     caLen:size_t{v caLen == aLen} -> a:lbignum aLen ->
     cbLen:size_t{v cbLen == bLen} -> b:lbignum bLen ->
-    i:size_t{v i <= aLen} ->
-    res:lbignum aLen -> Stack uint64
+    i:size_t{v i <= aLen} -> carry:uint64 ->
+    res:lbignum aLen -> Stack unit
     (requires (fun h -> live h a /\ live h b /\ live h res))
     (ensures (fun h0 _ h1 -> preserves_live h0 h1 /\ modifies1 res h0 h1))
     
-let rec bn_sub_ #aLen #bLen caLen a cbLen b i res =
-    if (i =. size 0) then u64 0
-    else begin
-        let i1 = size_decr i in
-        let carry' = bn_sub_ #aLen #bLen caLen a cbLen b i1 res in
-        let t1 = a.(i1) in 
-        let t2 = if (i1 <. cbLen) then b.(i1) else u64 0 in
-        let res_i = sub_mod #U64 (sub_mod #U64 t1 t2) carry' in
-        res.(i1) <- res_i;
-        (if (eq_u64 carry' (u64 1)) then
-            (if (le_u64 t1 t2) then u64 1 else u64 0)
-        else
-            (if (lt_u64 t1 t2) then u64 1 else u64 0))
+let rec bn_sub_ #aLen #bLen caLen a cbLen b i carry res =
+    if (i <. caLen) then begin
+       let t1 = a.(i) in
+       let t2 = if (i <. cbLen) then b.(i) else u64 0 in
+       let res_i = sub_mod #U64 (sub_mod #U64 t1 t2) carry in
+       res.(i) <- res_i;
+       let carry =
+           if (eq_u64 carry (u64 1)) then
+              (if (le_u64 t1 t2) then u64 1 else u64 0)
+           else
+              (if (lt_u64 t1 t2) then u64 1 else u64 0) in
+       bn_sub_ #aLen #bLen caLen a cbLen b (size_incr i) carry res
     end
 
 (* a must be greater than b *)
@@ -43,31 +42,28 @@ val bn_sub:
     res:lbignum aLen -> Stack unit
     (requires (fun h -> live h a /\ live h b /\ live h res))
     (ensures (fun h0 _ h1 -> preserves_live h0 h1 /\ modifies1 res h0 h1))
-    
-let bn_sub #aLen #bLen caLen a cbLen b res =
-    let _ = bn_sub_ #aLen #bLen caLen a cbLen b caLen res in ()
 
+let bn_sub #aLen #bLen caLen a cbLen b res =
+    bn_sub_ #aLen #bLen caLen a cbLen b (size 0) (u64 0) res
 
 val bn_add_:
     #aLen:size_nat -> #bLen:size_nat ->
     caLen:size_t{v caLen == aLen} -> a:lbignum aLen ->
     cbLen:size_t{v cbLen == bLen} -> b:lbignum bLen ->
-    i:size_t{v i <= aLen} ->
+    i:size_t{v i <= aLen} -> carry:uint64 ->
     res:lbignum aLen -> Stack uint64
     (requires (fun h -> live h a /\ live h b /\ live h res))
     (ensures (fun h0 _ h1 -> preserves_live h0 h1 /\ modifies1 res h0 h1))
     
-let rec bn_add_ #aLen #bLen caLen a cbLen b i res =
-    if (i =. size 0) then u64 0
-    else begin
-        let i1 = size_decr i in
-        let carry' = bn_add_ #aLen #bLen caLen a cbLen b i1 res in
-        let t1 = a.(i1) in 
-        let t2 = if (i1 <. cbLen) then b.(i1) else u64 0 in
-        let res_i = add_mod #U64 (add_mod #U64 t1 t2) carry' in
-        res.(i1) <- res_i;
-        (if (lt_u64 res_i t1) then u64 1 else u64 0)
-    end
+let rec bn_add_ #aLen #bLen caLen a cbLen b i carry res =
+    if (i <. caLen) then begin
+       let t1 = a.(i) in
+       let t2 = if (i <. cbLen) then b.(i) else u64 0 in
+       let res_i = add_mod #U64 (add_mod #U64 t1 t2) carry in
+       res.(i) <- res_i;
+       let carry = if (lt_u64 res_i t1) then u64 1 else u64 0 in
+       bn_add_ #aLen #bLen caLen a cbLen b (size_incr i) carry res end
+    else carry
 
 val bn_add:
     #aLen:size_nat -> #bLen:size_nat ->
@@ -76,8 +72,9 @@ val bn_add:
     res:lbignum aLen -> Stack unit
     (requires (fun h -> live h a /\ live h b /\ live h res))
     (ensures (fun h0 _ h1 -> preserves_live h0 h1 /\ modifies1 res h0 h1))
+
 let bn_add #aLen #bLen caLen a cbLen b res =
-    let _ = bn_add_ #aLen #bLen caLen a cbLen b caLen res in ()
+    let _ = bn_add_ #aLen #bLen caLen a cbLen b (size 0) (u64 0) res in ()
 
 val bn_add_carry:
     #aLen:size_nat -> #bLen:size_nat ->
@@ -89,5 +86,5 @@ val bn_add_carry:
     
 let bn_add_carry #aLen #bLen caLen a cbLen b res =
     let res' = Buffer.sub #uint64 #(aLen + 1) #aLen res (size 0) caLen in
-    let carry = bn_add_ #aLen #bLen caLen a cbLen b caLen res' in
+    let carry = bn_add_ #aLen #bLen caLen a cbLen b (size 0) (u64 0) res' in
     res.(caLen) <- carry
